serialize tags proof [skip ci]

src/Lib/DWT/ExecBer_tlv_tag_serialize.v
@@ -1,80 +1,133 @@
 Require Import VST.floyd.proofauto.
 Require Import Core.Core Core.Notations.
 
-Definition byte_length z :=
-  let fix byte_length n z i l :=
-      match n with
-      | O => l
-      | S n => if z >> i =? 0
-               then l 
-               else byte_length n z (i + 7) (l + 1)
-      end in
-  byte_length 4%nat z 7 1.
-
-Definition serialize_tag tval :=
-let fix serialize_tag n i tval :=
-  match n with
-  | O => [tval & 127]
-  | S n => (128 or (tval >> i & 127)) :: serialize_tag n (i - 7) tval
-  end in 
- let req_size := byte_length tval in 
- serialize_tag (Z.to_nat (req_size - 1)) ((req_size * 7) - 7)%Z tval.
-    
-Definition ber_tlv_tag_serialize (tag size : Z): list byte * Z :=
-  let tclass := tag & 3 in 
-  let tval := tag >> 2 in
-  if tval <=? 30 then (* Encoded in 1 octet *)
-    if eq_dec size 0 
-    then ([], 1)
-    else ([Byte.repr ((tclass << 6) or tval)], 1) 
-  else (* Encoded in > 1 octet *) 
-    let required_size := byte_length tval in
-    if eq_dec size 0 
-       then ([], required_size + 1)
-       else let buf0 := (tclass << 6) or 31 in
-            if size - 1 <? required_size 
-            then ([Byte.repr buf0], required_size + 1)
-            else
-            (map Byte.repr (buf0 :: (serialize_tag tag)), required_size + 1).
-
 Open Scope IntScope.
 
-Fixpoint byte_length'_loop n z i l :=
+Fixpoint required_size_loop n z l :=
   match n with
   | O => l
-  | S n => if Int.shru z i == 0
+  | S n => if z >>u (Int.repr l) * (Int.repr 7) == 0
           then l 
-          else byte_length'_loop n z (i + Int.repr 7) (l + 1)
+          else required_size_loop n z (l + 1)%Z
   end.
 
-Definition byte_length' z := byte_length'_loop 4%nat z (Int.repr 7) 1.
+Definition required_size z := required_size_loop 4%nat z 1%Z. 
 
-Fixpoint serialize_tag_loop  n i tval :=
+Lemma required_size_spec:
+         forall l : int, forall i : Z,
+           i = 1%Z \/ i = 2 \/ i = 3 \/ i = 4 \/ i = 5 ->
+           (forall j : Z, 0 <= j < i -> 
+               (l >>u (Int.repr j) * (Int.repr 7)) == 0 = false) ->
+                 l >>u (Int.repr i) * (Int.repr 7) = 0 -> 
+           required_size l = i.
+Proof.
+  intros l i N B SH.
+  repeat break_or_hyp.
+  * unfold required_size.
+      cbn in *.
+      rewrite SH.
+      replace (0 == 0) with true by reflexivity;
+      auto.
+  * unfold required_size.
+      cbn.
+    do 1 erewrite B.
+    autorewrite with norm in *.
+    cbn in *.
+    rewrite SH;
+      replace (0 == 0) with true by reflexivity;
+      auto.
+    normalize.
+    nia.
+  * unfold required_size;
+      cbn.
+    erewrite B.
+    erewrite B.
+     autorewrite with norm in *;
+    cbn in *;
+    rewrite SH;
+      replace (0 == 0) with true by reflexivity;
+      auto.
+    all: normalize;
+    nia.
+  * unfold required_size;
+      cbn.
+    erewrite B.
+    erewrite B.
+    erewrite B.
+     rewrite SH;
+      replace (0 == 0) with true by reflexivity;
+      auto.
+    all: nia.
+  * unfold required_size;
+      cbn.
+    erewrite B.
+    erewrite B.
+    erewrite B.
+     erewrite B.
+    all: nia.
+Qed.
+
+
+Fixpoint serialize_tag_loop s n t :=
   match n with
   | O => []
-  | S n => (Int.repr 128 or (Int.shru  tval (i & Int.repr 127))) 
-            :: serialize_tag_loop n (i - Int.repr 7) tval
+  | S n => 
+     let b := Int.zero_ext 8
+              (Int.repr 128 or 
+                        ((t >>u Int.repr (s * 7)) & Int.repr 127)) in
+     serialize_tag_loop (s + 1)%Z n t ++ [b]
   end. 
 
-Definition serialize_tag' tval :=
-  let s := byte_length' tval in 
-  let n := Z.to_nat (Int.unsigned (s - 1)) in
-  serialize_tag_loop n (s * Int.repr  7 - Int.repr 7) tval
-                     ++[(tval >> Int.repr 2) & Int.repr 127]. 
+Definition serialize_tag l := 
+  let s := required_size l in
+  let n := Z.to_nat s in
+  serialize_tag_loop 0%Z n l ++ [Int.zero_ext 8 (l & Int.repr 127)].
 
-Definition ber_tlv_tag_serialize' (tag size : int): list int * int :=
-  let tclass := tag & Int.repr 3 in 
-  let tval := Int.shru tag (Int.repr 2) in
-  if tval <=u Int.repr 30 then
-    if eq_dec size 0 
+Lemma loop_len_req_size : forall n l i, 
+    len (serialize_tag_loop i n l) = Z.of_nat n.
+        induction n; intros.
+          - reflexivity.
+          - simpl.
+            erewrite Zlength_app.
+            erewrite IHn.
+            cbn.
+            nia.
+Qed.
+           
+Lemma req_size_32 : forall l, 0 <= required_size l <= 5.
+Proof.
+  intros.
+  unfold required_size.
+  cbn.
+  repeat break_if; autorewrite with norm; nia.
+Qed.
+
+Open Scope Z.
+
+Definition ber_tlv_tag_serialize (tag size : int): list int * Z :=
+  let tclass := (tag & Int.repr 3)%int in 
+  let tval := tag >>u (Int.repr 2) in
+  if 30 >=? Int.unsigned tval then
+    if eq_dec size 0%int 
     then ([], 1)
-    else ([(tclass << Int.repr 6) or tval], 1) 
+    else ([Int.zero_ext 8 ((tclass << Int.repr 6) or tval)]%int, 1)
   else 
-    let required_size := byte_length' tval in
-    if eq_dec size 0 
-       then ([], required_size + 1)
-       else let buf0 := (tclass << Int.repr 6) or Int.repr 31 in
-            if (size - 1 <u required_size)
-            then ([buf0], required_size + 1)
+    let r := required_size tval in
+    if eq_dec size 0%int 
+       then ([], r + 1)
+       else let t := (Int.zero_ext 8 ((tclass << Int.repr 6) or Int.repr 31))%int in
+            if Int.unsigned size - 1 <? r
+            then ([t], r + 1)
             else
-            (buf0 :: (serialize_tag' tag), required_size + 1).
+            (t :: (serialize_tag tval), r + 1).
+
+Lemma shr_lt_zero_35: 
+             forall x, Int.shru x (Int.repr 35)
+                  = if Int.ltu x Int.zero then Int.mone else Int.zero.
+Proof.
+  intros. apply Int.same_bits_eq; intros.
+  rewrite Int.bits_shru; auto.
+  rewrite Int.unsigned_repr.
+  transitivity (Int.testbit x (Int.zwordsize - 1)).
+  f_equal. 
+Admitted.
