src/Lib/DWT/VSTber_tlv_tag_serialize.v
@@ -1,5 +1,7 @@
-Require Import Core.Core  Core.VstTactics Core.StructNormalizer VstLib DWT.Exec 
+Require Import Core.Core Core.VstTactics Core.StructNormalizer VstLib
         ErrorWithWriter.
+Require Import Core.Tactics.
+               
 Require Import VST.floyd.proofauto.
 Require Import Clight.ber_tlv_tag ExecBer_tlv_tag_serialize.
 Require Import Core.Notations Core.SepLemmas.
@@ -7,63 +9,60 @@ Require Import Core.Notations Core.SepLemmas.
 Instance CompSpecs : compspecs. Proof. make_compspecs prog. Defined.
 Definition Vprog : varspecs. Proof. mk_varspecs prog. Defined.
 
-Open Scope IntScope.
+Open Scope Z.
 
-Definition ber_tlv_tag_serialize_spec' : ident * funspec :=
+Definition ber_tlv_tag_serialize_spec : ident * funspec :=
   DECLARE _ber_tlv_tag_serialize
-  WITH tag : int, buf_b : block, buf_ofs : ptrofs, size : int, buf_size : Z
+  WITH tag : int, buf_b : block, buf_ofs : ptrofs, size : Z
   PRE[tuint, tptr tvoid, tuint]
-    PROP((32 <= buf_size)%Z)
-    PARAMS(Vint tag; (Vptr buf_b buf_ofs); Vint size)
+    PROP(32 < size < Int.modulus;
+         Ptrofs.unsigned buf_ofs + size < Ptrofs.modulus)
+    PARAMS(Vint tag; (Vptr buf_b buf_ofs); Vint (Int.repr size))
     GLOBALS()
-    SEP(data_at Tsh (tarray tuchar buf_size)
-                    (default_val (tarray tuchar buf_size)) 
+    SEP(data_at Tsh (tarray tuchar size)
+                    (default_val (tarray tuchar size)) 
                     (Vptr buf_b buf_ofs))
   POST[tuint]
-    let (ls, z) := ber_tlv_tag_serialize' tag size in
+    let (ls, z) := ber_tlv_tag_serialize tag (Int.repr size) in
     PROP()
-    LOCAL(temp ret_temp (Vint z))
+    LOCAL(temp ret_temp (Vint (Int.repr z)))
     SEP(if eq_dec ls [] 
-        then data_at Tsh (tarray tuchar buf_size)
-                         (default_val (tarray tuchar buf_size))
+        then data_at Tsh (tarray tuchar size)
+                         (default_val (tarray tuchar size))
                          (Vptr buf_b buf_ofs) 
-        else data_at Tsh (tarray tuchar buf_size)
-                         (map (fun x => Vint (Int.zero_ext 8 x)) ls ++ sublist (len ls) buf_size 
-                             (default_val (tarray tuchar buf_size)))
+        else data_at Tsh (tarray tuchar size)
+                         (map Vint ls ++ sublist (len ls) size 
+                             (default_val (tarray tuchar size)))
                          (Vptr buf_b buf_ofs)).
 
+Definition Gprog := ltac:(with_library prog [ber_tlv_tag_serialize_spec]).
 
-Definition Gprog' := ltac:(with_library prog [ber_tlv_tag_serialize_spec']).
+Open Scope IntScope.
 
-
-Theorem ber_tlv_tag_serialize_correct' : 
-  semax_body Vprog Gprog' (normalize_function f_ber_tlv_tag_serialize composites)
-             ber_tlv_tag_serialize_spec'.
+Theorem ber_tlv_tag_serialize_correct : 
+  semax_body Vprog Gprog (normalize_function f_ber_tlv_tag_serialize composites)
+             ber_tlv_tag_serialize_spec.
 Proof.
   start_function.
-  remember (tag >> Int.repr 2) as tval.
+  remember (Int.shru tag (Int.repr 2)) as tval.
   remember (Int.zero_ext 8 (((tag & Int.repr 3) << Int.repr 6) or tval)) as e0. 
-  remember (default_val (tarray tuchar buf_size)) as default_list.
+  remember (default_val (tarray tuchar size)) as default_list.
   remember (Int.zero_ext 8 (((tag & Int.repr 3) << Int.repr 6) or Int.repr 31)) as e1.
-  assert (len default_list = buf_size) as LB.
+  assert (len default_list = size) as LB.
   {  subst; unfold default_val;
         simpl;
         try erewrite Zlength_list_repeat;
         try nia; auto. }
+  pose proof (req_size_32 tval) as R.
   repeat forward.
   forward_if.
-  assert (((Int.shru tag (Int.repr 2)) <=u Int.repr 30) = true) as C.
-  { unfold Int.ltu.
-    break_if;
-    autorewrite with norm in *; try nia.
-    auto.  }
   - forward_if (
        PROP()
        LOCAL()
-       SEP(if eq_dec size 0 
-           then data_at_ Tsh (tarray tuchar buf_size) (Vptr buf_b buf_ofs) 
-           else data_at Tsh (tarray tuchar buf_size)
-                        (upd_Znth 0 (default_val (tarray tuchar buf_size))
+       SEP(if eq_dec (Int.repr size) 0 
+           then data_at_ Tsh (tarray tuchar size) (Vptr buf_b buf_ofs) 
+           else data_at Tsh (tarray tuchar size)
+                        (upd_Znth 0 (default_val (tarray tuchar size))
                                   (Vint e0)) (Vptr buf_b buf_ofs))).
     + forward. 
       rewrite_if_b.
@@ -75,38 +74,35 @@ Proof.
       unfold abbreviate. 
       break_let.
       forward.
-      break_if; unfold ber_tlv_tag_serialize' in *; rewrite C in *;
-        rewrite_if_b.
+     break_if; unfold ber_tlv_tag_serialize in *;
+     repeat rewrite_if_b;
+     eapply Z.ge_le in H1;
+     eapply Z.geb_le in H1;
+     rewrite H1 in *.
       * inversion Heqp.
         rewrite_if_b.
-        entailer!.               
+        entailer!.           
       * inversion Heqp.
         rewrite if_false by congruence.
         erewrite upd_Znth_unfold.
         rewrite LB.
         entailer!.
         nia.
-  - (* 30 < tag *)
-    assert (((tag >> Int.repr 2) <=u Int.repr 30) = false) as C.
-    
-    { unfold Int.ltu.
-      break_if;
-        autorewrite with norm in *; try nia.
-      auto.  }   
+  - (* 30 < tag *) 
     forward_if (
        PROP()
-       LOCAL(if eq_dec size 0 
+       LOCAL(if eq_dec (Int.repr size) 0 
              then temp _buf__1 (Vptr buf_b buf_ofs)
-             else temp _buf__1 (offset_val 1 (Vptr buf_b buf_ofs))  ;
-             if eq_dec size 0 
-             then temp _size (Vint size)
-             else temp _size (Vint (size - 1));
+             else temp _buf__1 (offset_val 1 (Vptr buf_b buf_ofs));
+             if eq_dec (Int.repr size) 0 
+             then temp _size (Vint (Int.repr size))
+             else temp _size (Vint (Int.repr (size - 1)));
             temp _tval (Vint tval))
-       SEP(if eq_dec size 0 
-           then data_at Tsh (tarray tuchar buf_size)
-                     (default_val (tarray tuchar buf_size)) (Vptr buf_b buf_ofs)  
-           else data_at Tsh (tarray tuchar buf_size)
-                        (upd_Znth 0 (default_val (tarray tuchar buf_size))
+       SEP(if eq_dec (Int.repr size) 0 
+           then data_at Tsh (tarray tuchar size)
+                     (default_val (tarray tuchar size)) (Vptr buf_b buf_ofs)  
+           else data_at Tsh (tarray tuchar size)
+                        (upd_Znth 0 (default_val (tarray tuchar size))
                                   (Vint e1)) (Vptr buf_b buf_ofs))).
     + rewrite <- LB.     
       erewrite split_data_at_sublist_tuchar with (j := 1%Z).
@@ -116,13 +112,15 @@ Proof.
       repeat forward.
       repeat rewrite_if_b.
       entailer!.
+      setoid_rewrite LB.
+      auto.
       erewrite upd_Znth_unfold.
       erewrite sublist_nil.
       erewrite app_nil_l.
-      remember (default_val (tarray tuchar buf_size)) as default_list.
+      remember (default_val (tarray tuchar size)) as default_list.
       remember (Int.zero_ext 8 (((tag & Int.repr 3) << Int.repr 6) or Int.repr 31)) as e1.     
       erewrite <- split_non_empty_list with
-          (j1 := buf_size)
+          (j1 := size)
           (ls :=  ([Vint e1] ++ sublist 1 (len default_list) default_list)).
       entailer!.
       reflexivity.
@@ -131,303 +129,562 @@ Proof.
         simpl;
         try erewrite Zlength_list_repeat;
         try nia; auto.
-      all: admit.
+      all: autorewrite with sublist;
+      try erewrite Zlength_sublist_correct;
+          try nia;  try setoid_rewrite LB; try nia.
     + forward.
       repeat rewrite_if_b.
       entailer!.
-    + (* loop *)
-      break_if.
+    + break_if.
+      assert ((30 >=? Int.unsigned (tag >>u Int.repr 2)) = false) as C.
+           { erewrite Z.geb_leb. 
+             Zbool_to_Prop.
+             nia. }
       ++ repeat forward.        
          forward_loop 
-      (EX i j: int, 
-          PROP ()
-          LOCAL (temp _tval (Vint (tag >> Int.repr 2));
-                 temp _i (Vint i);
-                 temp _required_size (Vint j);
-                 temp _size (Vint size);
+      (EX i: Z, 
+          PROP (i = 1%Z \/ i = 2 \/ i = 3 \/ i = 4 \/ i = 5; 
+                forall j, 0 <= j < i ->
+                     (Int.shru tval (Int.repr j * Int.repr 7) == 0)%int = false)
+          LOCAL (temp _tval (Vint (Int.shru tag (Int.repr 2)));
+                 temp _i (Vint (Int.repr (i * 7)));
+                 temp _required_size (Vint (Int.repr i));
+                 temp _size (Vint (Int.repr size));
                  temp _buf__1 (Vptr buf_b buf_ofs))
-          SEP (data_at Tsh (tarray tuchar buf_size)
-                       (default_val (tarray tuchar buf_size)) (Vptr buf_b buf_ofs)))
-      break: (EX i: int, 
-                 PROP (((tag >> Int.repr 2) >> i == 0)%int = true 
-                       \/ Int.unsigned i >= 8 * sizeof tuint)
-                 LOCAL (temp _required_size (Vint (byte_length' tval));
-                       temp _tval (Vint (tag >> Int.repr 2));
-                       temp _i (Vint i);
-                       temp _size (Vint size);
-                       temp _buf__1 (Vptr buf_b buf_ofs))
-                 SEP (data_at Tsh (tarray tuchar buf_size)
-                              (default_val (tarray tuchar buf_size)) (Vptr buf_b buf_ofs))).
-         * (* Pre implies Inv *)
-           Exists (Int.repr 7).
-           Exists 1.
+          SEP (data_at Tsh (tarray tuchar size)
+                       (default_val (tarray tuchar size))
+                       (Vptr buf_b buf_ofs)))
+      break: (let r := required_size (tag >>u(Int.repr 2)) in
+              PROP ()
+              LOCAL (temp _required_size (Vint (Int.repr r));
+                     temp _tval (Vint (tag >>u Int.repr 2));
+                     temp _i (Vint (Int.repr (r * 7)));
+                     temp _size (Vint (Int.repr size));
+                     temp _buf__1 (Vptr buf_b buf_ofs))
+                 SEP (data_at Tsh (tarray tuchar size)
+                              default_list
+                              (Vptr buf_b buf_ofs))).
+         * Exists 1%Z.
            entailer!.
-         * (* Inv exec fn Break *)
-           Intros i j.
+           intros. 
+           replace x with 0%Z by nia.
+           erewrite Int.shru_zero.
+           destruct  (Int.shru tag (Int.repr 2) == 0) eqn : T.
+           eapply int_eq_e in T.
+           rewrite T in H1.
+           cbv in H1.
+           congruence.
+           auto.
+         * Intro i.
            forward_if; repeat forward.
            forward_if;
             repeat forward.
-           Exists (i + Int.repr 7).
-           Exists (j + 1).
+           rewrite Int.unsigned_repr_eq in H2.
+           rewrite Zmod_small in H2.
            entailer!.
-           Exists i.
+           rep_omega.
+           Exists (i + 1)%Z.
+           rewrite Int.unsigned_repr_eq in H2.
+           rewrite Zmod_small in H2; try rep_omega.
            entailer!.
-           rewrite H2.
-           admit. (* need to replace j *)
-           Exists i.
-           entailer!.
-           admit.
+           split.
+        ** intros.
+           destruct (zeq j i).
+           subst.
+           eapply Int.eq_false.
+           autorewrite with norm.
+           eassumption.
+           eapply H4.
+           nia.
+        ** do 2 f_equal.
+           nia.
+        ** entailer!.
+           assert (required_size (tag >>u (Int.repr 2)) = i) as RS.
+           eapply required_size_spec; auto.
+           autorewrite with norm.
+           eassumption.
+           subst.
+           intuition.
+        ** entailer!.
+           rewrite Int.unsigned_repr_eq in H2.
+           rewrite Zmod_small in H2; try rep_omega.
+           replace i with 5 in * by nia.
+           assert (required_size (tag >>u (Int.repr 2)) = 5) as RS.
+           eapply required_size_spec; auto.
+           autorewrite with norm.
+           cbn.
+           erewrite shr_lt_zero_35.
+           break_if; auto.
+           unfold Int.ltu in Heqb.
+           break_if; autorewrite with norm in *.
+           replace (Int.unsigned 0) with 0%Z in * by auto with ints.
+           nia.
+           congruence.
+           rewrite RS.
+           intuition.
          * (* Post exec rest of the fn *)
-           Intros i.
+           simpl. 
            forward_if.
            unfold POSTCONDITION.
            unfold abbreviate. 
            break_let.
            forward.
-            unfold ber_tlv_tag_serialize' in *; rewrite C in *;
-              inversion Heqp;
-              rewrite_if_b.
+           unfold ber_tlv_tag_serialize in *.
+           rewrite C in *.
+           repeat rewrite_if_b.          
+           inversion Heqp.
            entailer!.
-           eapply ltu_false_inv in H2.
-           rewrite e in H2.
-           replace (Int.unsigned 0) with 0%Z in * by auto with ints. 
-           assert (1 <= Int.unsigned (byte_length' tval))%Z as BL.
-           { unfold byte_length'.
-             unfold byte_length'_loop.
-             repeat break_if; discriminate. }
-           nia.
-     ++ repeat forward.        
-         forward_loop 
-      (EX i j: int, 
-          PROP ()
-          LOCAL (temp _tval (Vint (tag >> Int.repr 2));
-                 temp _i (Vint i);
-                 temp _required_size (Vint j);
-                 temp _size (Vint (size - 1));
-                 temp _buf__1  (offset_val 1 (Vptr buf_b buf_ofs)))
-           SEP ((data_at Tsh (tarray tuchar buf_size)
-    (upd_Znth 0 (default_val (tarray tuchar buf_size)) (Vint e1)) (Vptr buf_b buf_ofs))))
-      break: (EX i: int, 
-                 PROP (((tag >> Int.repr 2) >> i == 0)%int = true 
-                       \/ Int.unsigned i >= 8 * sizeof tuint)
-                 LOCAL (temp _required_size (Vint (byte_length' tval));
-                       temp _tval (Vint (tag >> Int.repr 2));
-                       temp _i (Vint i);
-                       temp _size (Vint (size - 1));
-                       temp _buf__1  (offset_val 1 (Vptr buf_b buf_ofs)))
-                  SEP ((data_at Tsh (tarray tuchar buf_size)
-    (upd_Znth 0 (default_val (tarray tuchar buf_size))
-       (Vint e1)) (Vptr buf_b buf_ofs)))).
-         * (* Pre implies Inv *)
-           Exists (Int.repr 7).
-           Exists 1.
+           rewrite Int.unsigned_repr_eq in H2.
+           rewrite Zmod_small in H2; try rep_omega.           
+           assert (size = 0)%Z.
+           erewrite Int.int_to_unsigned_eq in e.
+           erewrite Int.unsigned_repr in e.
+           replace (Int.unsigned 0) with 0%Z in * by auto with ints.
+           auto.
+           rep_omega.
+           rep_omega.
+           rewrite Zmod_small in H2; try rep_omega.
+           subst.
+           rep_omega.
+           unfold Int.modulus.
+           unfold two_power_nat.
+           simpl.
+           subst. nia.
+           ++ repeat forward. 
+         forward_loop (EX i: Z, 
+          PROP (i = 1%Z \/ i = 2 \/ i = 3 \/ i = 4 \/ i = 5; 
+                forall j, 0 <= j < i ->
+                     (Int.shru tval (Int.repr j * Int.repr 7) == 0)%int = false)
+          LOCAL (temp _tval (Vint (tag >>u (Int.repr 2)));
+                 temp _i (Vint (Int.repr (i * 7)));
+                 temp _required_size (Vint (Int.repr i));
+                 temp _size (Vint (Int.repr (size - 1)));
+                 temp _buf__1 (offset_val 1 (Vptr buf_b buf_ofs)))
+          SEP ((data_at Tsh (tarray tuchar size)
+                        (upd_Znth 0 (default_val (tarray tuchar size))
+                                  (Vint e1)) (Vptr buf_b buf_ofs))))
+      break: (let r := required_size (tag >>u (Int.repr 2)) in
+              PROP ()
+              LOCAL (temp _required_size (Vint (Int.repr r));
+                     temp _tval (Vint (tag >>u Int.repr 2));
+                     temp _i (Vint (Int.repr (r * 7)));
+                     temp _size (Vint (Int.repr (size - 1)));
+                     temp _buf__1 (offset_val 1 (Vptr buf_b buf_ofs)))
+                 SEP ((data_at Tsh (tarray tuchar size)
+                               (upd_Znth 0 (default_val (tarray tuchar size)) 
+                                         (Vint e1)) (Vptr buf_b buf_ofs)))).
+         * Exists 1%Z.
            entailer!.
-         * (* Inv exec fn Break *)
-           Intros i j.
+           intros. 
+           replace x with 0%Z by nia.
+           erewrite Int.shru_zero.
+           destruct  (Int.shru tag (Int.repr 2) == 0) eqn : T.
+           eapply int_eq_e in T.
+           rewrite T in H1.
+           cbv in H1.
+           congruence.
+           auto.
+         * Intro i.
            forward_if; repeat forward.
            forward_if;
             repeat forward.
-           Exists (i + Int.repr 7).
-           Exists (j + 1).
+           rewrite Int.unsigned_repr_eq in H2.
+           rewrite Zmod_small in H2.
            entailer!.
-           Exists i.
+           rep_omega.
+           Exists (i + 1)%Z.
+           rewrite Int.unsigned_repr_eq in H2.
+           rewrite Zmod_small in H2; try rep_omega.
            entailer!.
-           rewrite H2.
-           admit. (* need to replace j *)
-           Exists i.
-           entailer!.
-           admit.
+           split.
+        ** intros.
+           destruct (zeq j i).
+           subst.
+           eapply Int.eq_false.
+           autorewrite with norm.
+           eassumption.
+           eapply H4.
+           nia.
+        ** do 2 f_equal.
+           nia.
+        ** entailer!.
+           assert (required_size (tag >>u (Int.repr 2)) = i) as RS.
+           eapply required_size_spec; auto.
+           autorewrite with norm.
+           eassumption.
+           subst.
+           intuition.
+        ** entailer!.
+           rewrite Int.unsigned_repr_eq in H2.
+           rewrite Zmod_small in H2; try rep_omega.
+           replace i with 5 in * by nia.
+           assert (required_size (tag >>u (Int.repr 2)) = 5) as RS.
+           eapply required_size_spec; auto.
+           autorewrite with norm.
+           cbn.
+           erewrite shr_lt_zero_35.
+           break_if; auto.
+           unfold Int.ltu in Heqb.
+           break_if; autorewrite with norm in *.
+           replace (Int.unsigned 0) with 0%Z in * by auto with ints.
+           nia.
+           congruence.
+           rewrite RS.
+           intuition.
          * (* Post exec rest of the fn *)
-           Intros i.
+            assert ((30 >=? Int.unsigned (tag >>u Int.repr 2)) = false) as C.
+           { erewrite Z.geb_leb. 
+             Zbool_to_Prop.
+             nia. }
+           simpl.
            forward_if.
            unfold POSTCONDITION.
            unfold abbreviate. 
            break_let.
            forward.
-           unfold ber_tlv_tag_serialize' in *; rewrite C in *;
-             rewrite_if_b.
-           entailer!.
-           rewrite H2 in *.
-           inversion Heqp.
-           reflexivity.
-           rewrite H2 in *.
-           inversion Heqp.
-           rewrite if_false by congruence.
-           entailer!.
-           erewrite upd_Znth_unfold.
-           erewrite sublist_nil.
-           erewrite app_nil_l.
-           replace (len (default_val (tarray tuchar buf_size))) with buf_size
-             by eassumption. 
-           entailer!.
-           nia.
+           unfold ber_tlv_tag_serialize in *.
+           rewrite C in *.
+           repeat rewrite_if_b.  
+           rewrite Int.unsigned_repr_eq in Heqp.
+           rewrite Zmod_small in Heqp; try rep_omega.
+           rewrite Int.unsigned_repr_eq in H2.
+           rewrite Zmod_small in H2; try rep_omega.
            forward.
            forward.
+           normalize.
+           autorewrite with norm.
+           Ltac unsig_repr := rewrite Int.unsigned_repr_eq;
+           rewrite Zmod_small; try rep_omega.
+           unsig_repr. 
+           remember (required_size tval) as r.
            forward_loop (
-               EX i : int, EX v : Z, EX ls : list int, 
-                           PROP ()
-                           LOCAL (temp _tval (Vint (tag >> Int.repr 2));
-                                  temp _i (Vint i);
-                                  temp _required_size (Vint (byte_length' tval));
-                                  temp _size (Vint (size - 1));
-                                  temp _buf__1 (offset_val (v + 1) (Vptr buf_b buf_ofs));
-                                  temp _end
-          (force_val (sem_binary_operation' Osub (tptr tuchar) tint
-             (eval_binop Oadd (tptr tuchar) tuint (offset_val 1 (Vptr buf_b buf_ofs)) 
-                         (Vint (byte_length' tval))) (Vint (Int.repr 1)))))
-          SEP (data_at Tsh (tarray tuchar 1) [Vint e1] (Vptr buf_b buf_ofs);
-               data_at Tsh (tarray tuchar v) (map Vint ls)
-                        (offset_val 1 (Vptr buf_b buf_ofs));
-               data_at Tsh (tarray tuchar (buf_size - v - 1)) 
-                                    (sublist (v + 1) buf_size default_list) 
+               EX v : Z, EX ls : list int,
+               PROP ((Int.unsigned Int.zero <= v)%Z; 
+                     (v <= r)%Z;
+                     ls = 
+                     serialize_tag_loop (r - v)%Z (Z.to_nat v) tval)
+               LOCAL (temp _tval (Vint tval);
+                      temp _i (Vint (Int.repr ((r * 7) - (v + 1) * 7)%Z));
+                      temp _required_size (Vint (Int.repr r));
+                      temp _size (Vint (Int.repr (size - 1)));
+                      temp _buf__1 (offset_val (v + 1) (Vptr buf_b buf_ofs));
+                      temp _end
+                      (Vptr buf_b
+                            (buf_ofs +
+                             Ptrofs.repr (1 + required_size (tag >>u Int.repr 2))
+                             - Ptrofs.repr 1)%ptrofs))
+               SEP (data_at Tsh (tarray tuchar 1) [Vint e1] (Vptr buf_b buf_ofs);
+                    data_at Tsh (tarray tuchar v) (map Vint ls)
+                            (offset_val 1 (Vptr buf_b buf_ofs));
+                    data_at Tsh (tarray tuchar (size - v - 1)) 
+                                    (sublist (v + 1) size default_list) 
                                     (offset_val (v + 1) (Vptr buf_b buf_ofs))))
+          break: (EX ls : list int, EX j: int, 
+                 PROP (let n := (Z.to_nat r) in
+                       ls = serialize_tag_loop 0 n tval)
+                 LOCAL (temp _tval (Vint (tag >>u Int.repr 2));
+                        temp _i (Vint j);
+                        temp _required_size (Vint (Int.repr r));
+                        temp _size (Vint (Int.repr (size - 1)));
+                        temp _buf__1 (offset_val (len ls + 1) (Vptr buf_b buf_ofs));
+                        temp _end
+                             (Vptr buf_b
+                                   (buf_ofs +
+                                    Ptrofs.repr (1 + 
+                                                 required_size (tag >>u Int.repr 2))
+                                    - Ptrofs.repr 1)%ptrofs))
 
-          break: (EX i: int, EX ls : list int,
-
-                       PROP (let s := byte_length' tag in 
-                             let n := Z.to_nat (Int.unsigned (s - 1)) in
-                             ls = serialize_tag_loop n
-                                (s * Int.repr  7 - Int.repr 7)%int tag)
-
-                       LOCAL (temp _tval (Vint (tag >> Int.repr 2));
-                              temp _i (Vint i);
-                              temp _required_size (Vint (byte_length' tval));
-                              temp _size (Vint (size - 1));
-                              temp _buf__1 (offset_val (len ls + 1) (Vptr buf_b buf_ofs)))
-
-                       SEP (data_at Tsh (tarray tuchar 1) [Vint e1] (Vptr buf_b buf_ofs);
-                            data_at Tsh (tarray tuchar (len ls)) 
-                                    (map (fun x : int => Vint (Int.zero_ext 8 x)) ls)
-                                    (offset_val 1 (Vptr buf_b buf_ofs));
-                            data_at Tsh (tarray tuchar buf_size) 
-                                    (sublist (len ls + 1) buf_size default_list) 
-                                    (offset_val ((Zlength ls) + 1) (Vptr buf_b buf_ofs)))).
-          *** Exists (i - Int.repr 7).
-              Exists 0%Z.
+                 SEP (data_at Tsh (tarray tuchar 1) [Vint e1] (Vptr buf_b buf_ofs);
+                      data_at Tsh (tarray tuchar (len ls)) 
+                              (map Vint ls)
+                              (offset_val 1 (Vptr buf_b buf_ofs));
+                      data_at Tsh (tarray tuchar (size - len ls - 1)) 
+                                    (sublist (len ls + 1) size default_list) 
+                                    (offset_val ((len ls) + 1) (Vptr buf_b buf_ofs)))).
+          *** Exists 0%Z.
               Exists (@nil int).
-              entailer!.
               erewrite data_at_tuchar_zero_array_eq.
               entailer!.
-              erewrite <- data_at_app2.
+              erewrite <- data_at_app.
               erewrite upd_Znth_unfold.
               erewrite sublist_nil.
               erewrite app_nil_l.
-              replace (len (default_val (tarray tuchar buf_size))) with buf_size.
+              replace (len (default_val (tarray tuchar size))) with size.
               entailer!.
-              replace (1 + (buf_size - 1))%Z with buf_size by nia.
+              replace (1 + (size - 1))%Z with size by nia.
               entailer!.
-              nia.
-              reflexivity.
-              autorewrite with sublist norm; auto.
-              cbn; auto.
-          *** Intros j v ls.
-              forward_if.
-              admit.
-              unfold tarray. 
-              erewrite split2_data_at_Tarray_tuchar with (n0 := (buf_size - v - 1)%Z)  (n1 := 1%Z).
-               erewrite sublist_one.
-              erewrite data_at_tuchar_singleton_array_eq at 1.
-              erewrite data_at_tuchar_singleton_array_eq at 1.
-              Intros.
-              forward.
-              entailer!.
-              admit.
-              repeat forward.              
-              Exists (j - Int.repr 7).
-              Exists (v + 1)%Z.
-              Exists (ls ++ [Int.repr 128 or ((tval >> j) & (Int.repr 127))]).
-              entailer!.
-              all: try nia.
-              1-4: admit.
-              forward.
-              Exists j.
-              Exists ls.
-              entailer!.
-              assert (len ls = v) by admit.              
-              subst.
-              admit.
-               assert (len ls = v) by admit.              
-              subst.
-              entailer!.
-              admit.
-          *** Intros i0 ls.
-              unfold offset_val.
-              erewrite split_non_empty_list
-                with (ls' := sublist (len ls + 1 + 1) buf_size default_list)
-                     (j2 := (buf_size - (len ls + 1 + 1))%Z)
-                     (ofs := (buf_ofs + Ptrofs.repr (len ls + 1))%ptrofs).
-              Intros.
-              forward.
-              unfold POSTCONDITION.
-              unfold abbreviate. 
-              break_let.
-              forward.
-              unfold ber_tlv_tag_serialize' in *; rewrite C in *;
-                rewrite_if_b.
-              rewrite H2 in *.
-              inversion Heqp.
-              rewrite_if_b.
-              rewrite if_false by congruence.               
-              unfold serialize_tag'.
-              rewrite <- H3.
-              clear H3.
-              entailer!.
-              remember (default_val (tarray tuchar buf_size)) as default_list.
-              remember (Int.zero_ext 8 (((tag & Int.repr 3) << Int.repr 6) or Int.repr 31)) as e1.
-              remember (Int.zero_ext 8 ((tag >> Int.repr 2) & Int.repr 127)) as e_n.
-              unfold offset_val.
-              simpl.
-              erewrite <- data_at_tuchar_singleton_array_eq.
-              erewrite <- data_at_app2.
-              replace (1 + len ls)%Z with (len ls + 1)%Z by nia.
-              erewrite <- data_at_app2.
-              replace (buf_ofs + Ptrofs.repr (len ls + 1) + 1)%ptrofs
-                with (buf_ofs + Ptrofs.repr (len ls + 1 + 1))%ptrofs.
-              erewrite <- data_at_app2.
-              replace ((len ls + 1 + 1 + (buf_size - (len ls + 1 + 1))))%Z
-                with buf_size.
-              assert (((([Vint e1] ++
-                         map (fun x : int => Vint (Int.zero_ext 8 x)) ls) ++ 
-                        [Vint e_n]) ++
-                        sublist (len ls + 1 + 1) buf_size default_list) =
-                       (Vint e1
-         :: map (fun x : int => Vint (Int.zero_ext 8 x))
-              (ls ++ [(tag >> Int.repr 2) & Int.repr 127]) ++
-            sublist
-              (len
-                 ((((tag & Int.repr 3) << Int.repr 6) or Int.repr 31)
-                  :: ls ++ [(tag >> Int.repr 2) & Int.repr 127])) buf_size default_list)).
-              replace  (len
-                 ((((tag & Int.repr 3) << Int.repr 6) or Int.repr 31)
-                  :: ls ++ [(tag >> Int.repr 2) & Int.repr 127])) with (len ls + 1 + 1)%Z by
-              (autorewrite with sublist list norm;
-              nia).
-              repeat erewrite map_app.
-              subst.
-              reflexivity.
-              subst.
-              entailer!.
-              nia.
-              all : (autorewrite with sublist list norm;
+              all: try setoid_rewrite LB;
+                autorewrite with sublist norm; cbn; auto;
+                  try rep_omega.
+          ***
+            Intros v ls.
+            forward_if.
+           +++
+             assert (0 <= v + 1 <= (required_size (tag >>u Int.repr 2))) as VR by admit.
+             unfold test_order_ptrs.
+             unfold sameblock.
+             subst.
+             destruct peq; [simpl  |contradiction].
+             apply andp_right.
+             { apply derives_trans 
+                 with (Q := valid_pointer 
+                              (Vptr buf_b (buf_ofs + Ptrofs.repr (v + 1))%ptrofs)).
+               entailer!.
+               apply valid_pointer_weak. }
+             { assert (0 < size - v - 1)%Z as LD by
+                     (try erewrite LB; nia).
+               assert (sizeof (tarray tuchar (size - v - 1)) > 0) by (simpl; nia).
+               remember (default_val (tarray tuchar size)) as default_list.
+               remember (required_size (tag >>u Int.repr 2)) as r.
+               assert (data_at Tsh (tarray tuchar (size - v - 1))
+                               (sublist (v + 1) size (default_val (tarray tuchar size)))
+                               (Vptr buf_b (buf_ofs + Ptrofs.repr (v + 1))%ptrofs)
+                               |-- weak_valid_pointer
+                               (Vptr buf_b
+                                     (buf_ofs +  Ptrofs.repr (1 + r) - Ptrofs.repr 1)%ptrofs)).
+               { apply derives_trans 
+                   with (Q := valid_pointer 
+                                (Vptr buf_b (buf_ofs
+                                             + Ptrofs.repr
+                                                 (1 + r) - Ptrofs.repr 1)%ptrofs)). 
+                 assert (sizeof (tarray tuchar (size - v - 1)) > 0) by (simpl; nia).
+                 replace (buf_ofs + Ptrofs.repr (1 + r) - Ptrofs.repr 1)%ptrofs
+                   with (buf_ofs + Ptrofs.repr r)%ptrofs.
+                 Open Scope Z.
+                 erewrite data_at_app_gen
+                   with (j1 := r - (v + 1))
+                        (j2 := len default_list - r)
+                        (ls1 := sublist (v + 1) r default_list)
+                        (ls2 := sublist r (len default_list) default_list). 
+                 assert ((buf_ofs + Ptrofs.repr (v + 1) + Ptrofs.repr (r - (v + 1)))%ptrofs =
+                         (buf_ofs + Ptrofs.repr r)%ptrofs) as PTR.
+                 {  ptrofs_compute_add_mul; try rep_omega.
+                    f_equal.
+                    rep_omega. }
+                 rewrite PTR.
+                 assert (sizeof (tarray tuchar (len default_list -  r)) > 0).
+                 { simpl.
+                   setoid_rewrite LB. 
+                   nia. }
+                 eapply sepcon_valid_pointer2.
+                 eapply data_at_valid_ptr; auto.
+                 1-5:  replace (Int.unsigned 0%int) with 0%Z in * by auto with ints.
+                 4: erewrite sublist_split with (mid := r); subst; auto; try nia.
+                 all: try erewrite Zlength_sublist_correct;
+                   try nia;  try setoid_rewrite LB; try nia; auto.
+                 Focus 3. apply valid_pointer_weak. 
+                 try erewrite Zlength_sublist_correct;
+                   try nia;  try setoid_rewrite LB; ptrofs_compute_add_mul; try rep_omega.
+                 erewrite Ptrofs.sub_add_opp.
+                 unfold Ptrofs.neg.
+                 normalize.
+                 f_equal.
+                 rewrite Ptrofs.unsigned_repr.
+                 f_equal.
+                 nia.
+                 rep_omega.  }
+               entailer!. }
+           +++
+             unfold offset_val.
+             erewrite split_non_empty_list with 
+                 (j2 := (len default_list - (v + 1) - 1)%Z)
+                 (ls' := (sublist (v + 1 + 1) size default_list))
+                 (ls := (sublist (v + 1) size default_list)).
+             eapply typed_true_ptr_lt in H6.
+             assert (v < required_size tval)%Z.
+             { replace (Int.unsigned 0%int) with 0 in * by auto with ints.
+               generalize H6.
+               unfold Ptrofs.sub.
+               ptrofs_compute_add_mul. 
+               all: subst; rep_omega_setup; auto with ints; 
+                 autorewrite with norm; try rep_omega; try nia.  }
+             Intros.
+             assert (len default_list - (v + 1) - 1 =
+                     len (sublist (v + 1 + 1) (len default_list) default_list)) as LEN.
+             { erewrite Zlength_sublist_correct.
+               nia.
+               rewrite LB.
+               replace (Int.unsigned 0%int) with 0%Z in * by auto with ints.
+               all: nia. }
+             forward.
+             entailer!.
+             unfold Int.iwordsize.
+             ints_compute_add_mul.
+             cbn - [required_size].
+             replace (Int.unsigned 0%int) with 0%Z in H4 by (autorewrite with norm; auto).   
+             all: try rep_omega.
+             repeat forward.
+             remember
+               (Int.zero_ext 8
+                             (Int.repr 128
+                                       or (((tag >>u Int.repr 2) >>u
+                                                                 Int.repr ((required_size (tag >>u Int.repr 2) - (len ls + 1)) * 7)) & Int.repr 127))%int)%int
+               as e_v.
+             Exists (v + 1) (ls ++ [e_v]).
+             assert (v = len ls) as VLS.
+             { subst.
+               erewrite loop_len_req_size.
+               replace (Int.unsigned 0%int) with 0%Z in * by (autorewrite with norm; auto).   
+               erewrite Z2Nat_id';
+                 erewrite Zmax0r; try nia. }
+             entailer!.
+             split.
+             erewrite Z.add_1_r at 3.
+             erewrite Z2Nat.inj_succ.       
+             simpl. f_equal. rewrite H5 at 1. 
+             replace (required_size (tag >>u Int.repr 2)  - len ls) 
+               with (required_size (tag >>u Int.repr 2)  - (len ls + 1) + 1) by nia.
+             reflexivity.
+             normalize.
+             do 2 f_equal. nia.
+             replace (required_size (tag >>u Int.repr 2) * 7 - (len ls + 1) * 7)
+               with
+                 ((required_size (tag >>u Int.repr 2) - (len ls + 1)) * 7) by nia.
+             remember
+               (Int.zero_ext 8
+                             (Int.repr 128
+                                       or (((tag >>u Int.repr 2) >>u
+                            Int.repr ((required_size (tag >>u Int.repr 2)
+                                       - (len ls + 1)) * 7)) & 
+                                           Int.repr 127))%int)%int
+               as e_v.
+             unfold offset_val.
+             simpl.
+             erewrite <- data_at_tuchar_singleton_array_eq.
+             remember (default_val (tarray tuchar size)) as default_list.
+             replace (buf_ofs + Ptrofs.repr (len ls + 1) + 1)%ptrofs
+               with (buf_ofs +  Ptrofs.repr (len ls + 1 + 1))%ptrofs. 
+             
+             replace (buf_ofs + Ptrofs.repr ((len ls) + 1))%ptrofs
+               with (buf_ofs + 1 + Ptrofs.repr (len ls))%ptrofs. 
+             erewrite <- data_at_app.
+             erewrite map_app.
+             rewrite <- LB.
+             entailer!.
+             all: replace (Int.unsigned 0%int) with 0%Z in * 
+               by (autorewrite with norm; auto);
+               autorewrite with list sublist;
+               try rep_omega.
+             all: ptrofs_compute_add_mul; 
+               replace (Ptrofs.unsigned 1%ptrofs) with 1 by auto with ptrofs;
+               autorewrite with norm;
+               try nia; try rep_omega; f_equal; try nia.
+             instantiate (1 := Znth (v + 1) default_list).
+             erewrite sublist_split with (mid := v + 1 + 1).
+             erewrite sublist_len_1.
+             reflexivity.
+             all: try setoid_rewrite LB; try nia.
+           +++
+             eapply typed_false_ptr_lt in H6.
+             assert (required_size tval < size) by nia.
+             assert (v + 1 >= required_size tval)%Z. 
+             { replace (Int.unsigned 0%int) with 0 in * by auto with ints.
+               generalize H6.
+               unfold Ptrofs.sub.
+               ptrofs_compute_add_mul. 
+                all: subst; rep_omega_setup; auto with ints; 
+                 autorewrite with norm; try rep_omega; try nia. }
+             repeat forward.
+             assert (v = r \/ v + 1 = r) as V by nia.
+             inversion V as [V1 | V2].
+             { rewrite V1.
+             rewrite Heqr.  
+             Exists ls (Int.repr ((r * 7) - (r + 1) * 7)%Z).
+             replace (required_size tval - required_size tval)%Z with 0%Z by nia.
+             entailer!.
+             split.
+             replace (required_size (tag >>u Int.repr 2) 
+                      - required_size (tag >>u Int.repr 2))%Z with 0%Z by nia.
+             reflexivity.
+             erewrite Zlength_map in H12.
+             setoid_rewrite H12.
+             reflexivity.
+             replace (required_size (tag >>u Int.repr 2) -
+                      required_size (tag >>u Int.repr 2))%Z with 0%Z in * by nia.
+             remember (tag >>u Int.repr 2) as tval.
+             remember (serialize_tag_loop 0 (Z.to_nat (required_size tval)) tval) as ls.
+             assert (required_size tval = len ls) as L.
+             {  erewrite Zlength_map in H12.
+                subst.
+                rewrite <- H12 at 1.
+                reflexivity. }
+             rewrite L.
+             entailer!. }
+            { 
+              Exists ls (Int.repr ((r * 7) - r * 7)%Z).
+              admit. }
+             *** 
+               Intros ls j.
+               unfold offset_val.
+               erewrite split_non_empty_list
+                 with (ls' := sublist (len ls + 1 + 1) size default_list)
+                      (j2 := (size - (len ls + 1 + 1))%Z)
+                      (ofs := (buf_ofs + Ptrofs.repr (len ls + 1))%ptrofs).
+               Intros.
+               forward.
+               unfold POSTCONDITION.
+               unfold abbreviate.
+               break_let.
+               pose proof (req_size_32 tval).
+               assert (required_size tval < size) by nia.
+               forward.
+               unfold ber_tlv_tag_serialize in *.
+               rewrite C in *.
+               rewrite Int.unsigned_repr_eq in *.
+               rewrite Zmod_small in *.
+               rewrite_if_b.
+                assert ((size - 1 <? required_size (tag >>u Int.repr 2)) = false) as S.
+                { Zbool_to_Prop.
+                  nia. }
+               rewrite S in *.
+               inversion Heqp.
+               unfold serialize_tag.
+               rewrite if_false by congruence.
+               unfold offset_val.                   
+               erewrite <- data_at_tuchar_singleton_array_eq.
+               erewrite <- data_at_app.
+               replace (1 + len ls)%Z with (len ls + 1)%Z by nia.
+               erewrite <- data_at_app.
+               setoid_rewrite <- H3.
+               remember (Int.zero_ext 8 (((tag & Int.repr 3)
+                                            << Int.repr 6) or Int.repr 31)%int) as e0.
+               remember (Int.zero_ext 8 ((tag >>u Int.repr 2) & Int.repr 127)%int) as e_n.
+               replace (buf_ofs + Ptrofs.repr (len ls + 1) + 1)%ptrofs with 
+                   (buf_ofs + Ptrofs.repr (len ls + 1 + 1))%ptrofs.
+               erewrite <- data_at_app.
+               replace (len ls + 1 + 1 + (size - (len ls + 1 + 1))) with size by nia.
+               autorewrite with sublist list norm.
+               erewrite map_app.
+               entailer!.
+               all: (autorewrite with sublist list norm;
                      try nia; auto).
-                erewrite Zlength_sublist_correct.
-              nia.
-              admit.
-              subst; try setoid_rewrite LB; try nia. 
-              admit.
-             (*  all: pose proof (Zlength_nonneg ls); try nia;
-                subst; try setoid_rewrite LB; try nia.   *)
-              erewrite sublist_split with (mid := (len ls + 1 + 1)%Z).
-              erewrite sublist_one.
-              reflexivity.
-              all: pose proof (Zlength_nonneg ls); try nia;
-                subst; try setoid_rewrite LB; try nia.     
-              admit.
-              admit.
-              admit.
-              erewrite Zlength_sublist_correct.
-              nia.
-              admit.
-              admit.
+               all: try erewrite Zlength_sublist_correct;
+                 try nia.
+               Focus 6.
+               instantiate (1 := Znth (len ls + 1) default_list).
+               erewrite sublist_split with (mid := len ls + 1 + 1).
+               erewrite sublist_len_1.
+               reflexivity.
+               all: try setoid_rewrite LB; try  rep_omega.
+               all: try setoid_rewrite LB;
+                 try (simpl in H3;
+                      subst;
+                      erewrite loop_len_req_size;
+                      erewrite Z2Nat_id';
+                      erewrite Zmax0r;
+                      repeat rep_omega).
+               all: try setoid_rewrite LB;
+                 try (simpl in H3;
+                      subst;
+                      erewrite loop_len_req_size;
+                      erewrite Z2Nat_id';
+                      erewrite Zmax0r;
+                      repeat rep_omega).
+               all: repeat ptrofs_compute_add_mul. 
+               replace (Ptrofs.unsigned 1%ptrofs) with 1%Z by auto with ptrofs.
+               f_equal.
+               nia.
+               all: subst; rep_omega_setup; auto with ints; 
+                 autorewrite with norm; try rep_omega; try nia.
+             *** subst. rep_omega.
 Admitted.
-
